src/tactics/FStar.Tactics.V2.Interpreter.fst
@@ -634,6 +634,18 @@ let () =
         ext_getns e_string (e_list (e_tuple2 e_string e_string))
         ext_getns NBET.e_string NBET.(e_list (e_tuple2 e_string e_string));
 
+      mk_tac_step_2 1 "alloc"
+        (fun _ -> alloc) e_any e_any (E.e_tref #S.term)
+        (fun _ -> alloc) NBET.e_any NBET.e_any (E.e_tref_nbe #NBET.t);
+
+      mk_tac_step_2 1 "read"
+        (fun _ -> read) e_any (E.e_tref #S.term) e_any
+        (fun _ -> read) NBET.e_any (E.e_tref_nbe #NBET.t) NBET.e_any;
+
+      mk_tac_step_3 1 "write"
+        (fun _ -> write) e_any (E.e_tref #S.term) e_any e_unit
+        (fun _ -> write) NBET.e_any (E.e_tref_nbe #NBET.t) NBET.e_any NBET.e_unit;
+
       // reflection typechecker callbacks (part of the DSL framework)
 
       mk_tac_step_2 0 "is_non_informative"
